{
 "cells": [
  {
   "cell_type": "code",
   "execution_count": null,
   "id": "017a1181",
   "metadata": {},
   "outputs": [],
   "source": [
    "import numpy as np\n",
    "import sympy as sp\n",
    "import scipy\n",
    "import os\n",
    "import time\n",
    "from  matplotlib import pyplot as plt"
   ]
  },
  {
   "cell_type": "markdown",
   "id": "ba6e2e33",
   "metadata": {},
   "source": [
    "### Show that the Lane-Emden equation can be derived by combining hydrostatic equilibrium, a polytropic equation of state and the continuity equation."
   ]
  },
  {
   "cell_type": "markdown",
   "id": "e616c1d5",
   "metadata": {},
   "source": [
    "Polytropic equation of state\n",
    "\n",
    "$$P=K\\rho^{1+\\frac1n}$$"
   ]
  },
  {
   "cell_type": "markdown",
   "id": "b8a786a3",
   "metadata": {},
   "source": [
    "Continuity equation\n",
    "\n",
    "$$\\frac{dm}{dr}=4\\pi r^2 \\rho$$"
   ]
  },
  {
   "cell_type": "markdown",
   "id": "92d6b97a",
   "metadata": {},
   "source": [
    "Tolman-Oppenheimer-Volkoff equation\n",
    "\n",
    "$$\\frac{dP}{dr} = -\\frac{Gm\\rho}{r^2}(1+\\frac{P}{\\rho c^2})(1+\\frac{4\\pi r^2 P}{mc^2})(1-\\frac{2Gm}{rc^2})^{-1}$$"
   ]
  },
  {
   "cell_type": "markdown",
   "id": "f9d845b5",
   "metadata": {},
   "source": [
    "Lane-Emden equation\n",
    "\n",
    "\n",
    "$$\\frac 1 {\\xi^2} \\frac d{d\\xi}(\\xi^2\\frac{d\\theta}{d\\xi}) + \\theta^n = 0$$"
   ]
  },
  {
   "cell_type": "markdown",
   "id": "a06445d3",
   "metadata": {},
   "source": [
    "## Hand working for n=0, solution for LE"
   ]
  },
  {
   "cell_type": "markdown",
   "id": "f122f1c1",
   "metadata": {},
   "source": [
    "$$\\frac 1 {\\xi^2} \\frac d{d\\xi}(\\xi^2\\frac{d\\theta}{d\\xi}) + 1 = 0$$"
   ]
  },
  {
   "cell_type": "markdown",
   "id": "3e88050e",
   "metadata": {},
   "source": [
    "$$\\frac d{d\\xi}(\\xi^2\\frac{d\\theta}{d\\xi}) = -\\xi^2$$"
   ]
  },
  {
   "cell_type": "markdown",
   "id": "0180411d",
   "metadata": {},
   "source": [
    "$$\\xi^2\\frac{d\\theta}{d\\xi} = \\int-\\xi^2 d\\xi$$"
   ]
  },
  {
   "cell_type": "markdown",
   "id": "b2136614",
   "metadata": {},
   "source": [
    "$$\\xi^2\\frac{d\\theta}{d\\xi} = C -\\frac13\\xi^3 $$"
   ]
  },
  {
   "cell_type": "markdown",
   "id": "20728567",
   "metadata": {},
   "source": [
    "$$\\frac{d\\theta}{d\\xi} = C -\\frac13\\xi $$"
   ]
  },
  {
   "cell_type": "markdown",
   "id": "8808e641",
   "metadata": {},
   "source": [
    "$${d\\theta} = C -\\frac13\\xi {d\\xi}$$"
   ]
  },
  {
   "cell_type": "markdown",
   "id": "6de3ee2a",
   "metadata": {},
   "source": [
    "$$\\theta(\\xi) = \\int [C -\\frac13\\xi ]{d\\xi}$$"
   ]
  },
  {
   "cell_type": "markdown",
   "id": "38e37f53",
   "metadata": {},
   "source": [
    "$$\\theta(\\xi) = D - \\frac C\\xi - \\frac16\\xi^2$$"
   ]
  },
  {
   "cell_type": "markdown",
   "id": "b83bee47",
   "metadata": {},
   "source": [
    "Apply initial conditions $\\theta(0) = 1, \\theta'(0) \\equiv \\frac{d\\theta}{d\\xi}|_{\\xi=0} = 0$"
   ]
  },
  {
   "cell_type": "markdown",
   "id": "e3cab19a",
   "metadata": {},
   "source": [
    "$$\\theta'(\\xi) = 0 = C - \\frac13 \\xi$$\n",
    "\n",
    "$$\\theta'(0) = 0 = C - \\frac13 0$$\n",
    "\n",
    "$$\\Rightarrow C = 0$$"
   ]
  },
  {
   "cell_type": "markdown",
   "id": "19b82e41",
   "metadata": {},
   "source": [
    "$$\\theta(0) = 1 = D - \\frac16 0$$\n",
    "\n",
    "$$\\Rightarrow D = 1$$"
   ]
  },
  {
   "cell_type": "markdown",
   "id": "7e77417f",
   "metadata": {},
   "source": [
    "$$\\theta(\\xi) = 1 - \\frac16\\xi^2$$"
   ]
  },
  {
   "cell_type": "markdown",
   "id": "849af023",
   "metadata": {},
   "source": [
    "## Hand working for n=1, solution for LE"
   ]
  },
  {
   "cell_type": "markdown",
   "id": "1087cc38",
   "metadata": {},
   "source": [
    "$$\\frac 1 {\\xi^2} \\frac d{d\\xi}(\\xi^2\\frac{d\\theta}{d\\xi}) + \\theta = 0$$"
   ]
  },
  {
   "cell_type": "markdown",
   "id": "2fb2010d",
   "metadata": {},
   "source": [
    "By the chain rule\n",
    "\n",
    "$$\\frac{d^2\\theta}{d\\xi^2} + \\frac2\\xi\\frac{d\\theta}{d\\xi} + \\theta = 0$$"
   ]
  },
  {
   "cell_type": "markdown",
   "id": "5246b2a4",
   "metadata": {},
   "source": [
    "Trying the Fourier transform to solve the 2nd order ODE\n",
    "\n",
    "$$\\theta''(\\xi) + \\frac2\\xi \\theta'(\\xi) + \\theta(\\xi) = 0$$"
   ]
  },
  {
   "cell_type": "markdown",
   "id": "030ef6ba",
   "metadata": {},
   "source": [
    "Using the substitution that $\\theta(\\xi) = \\frac{u(\\xi)}{\\xi}$\n",
    "\n",
    "$$\\theta(\\xi) = \\frac{u(\\xi)}{\\xi}$$\n",
    "$$\\theta'(\\xi) = \\frac{u'(\\xi)\\xi - u(\\xi)}{\\xi^2}$$\n",
    "$$= \\frac{u'(\\xi)\\xi}{\\xi^2} - \\frac{u(\\xi)}{\\xi^2}$$\n",
    "$$= \\frac{u'(\\xi)}{\\xi} - \\frac{u(\\xi)}{\\xi^2}$$\n",
    "\n",
    "$$\\theta''(\\xi) = \\frac {u''(\\xi)\\xi - u'(\\xi)}{\\xi^2} - \\frac{u'(\\xi)\\xi^2 - 2\\xi u(\\xi)}{\\xi^4}$$\n",
    "$$\\theta''(\\xi) = \\frac{u''(\\xi)}{\\xi} - \\frac{u'(\\xi)}{\\xi^2} - \\frac{u'(\\xi)\\xi^2}{\\xi^4} + \\frac{2\\xi u(\\xi)}{\\xi^4}$$\n",
    "$$\\theta''(\\xi) = \\frac{u''(\\xi)}{\\xi} - \\frac{2u'(\\xi)}{\\xi^2} + \\frac{2u(\\xi)}{\\xi^3}$$\n"
   ]
  },
  {
   "cell_type": "markdown",
   "id": "77f0bc12",
   "metadata": {},
   "source": [
    "Applying the substitution\n",
    "\n",
    "$$\\theta''(\\xi) + \\frac2\\xi \\theta'(\\xi) + \\theta(\\xi) = 0$$\n",
    "\n",
    "becomes\n",
    "\n",
    "$$\\frac{u''(\\xi)}{\\xi} - \\frac{2u'(\\xi)}{\\xi^2} + \\frac{2u(\\xi)}{\\xi^3} + \\frac2\\xi(\\frac{u'(\\xi)}{\\xi} - \\frac{u(\\xi)}{\\xi^2}) + \\frac{u(\\xi)}{\\xi} = 0$$\n",
    "$$\\frac{u''(\\xi)}{\\xi} - \\frac{2u'(\\xi)}{\\xi^2} + \\frac{2u(\\xi)}{\\xi^3} +\\frac{2u'(\\xi)}{\\xi^2} - \\frac{2u(\\xi)}{\\xi^3} + \\frac{u(\\xi)}{\\xi} = 0$$\n",
    "$$\\frac{u''(\\xi)}{\\xi} + \\frac{u(\\xi)}{\\xi} = 0$$\n",
    "\n",
    "Multiply by $\\xi$\n",
    "\n",
    "$$u''(\\xi) + u(\\xi) = 0$$"
   ]
  },
  {
   "cell_type": "markdown",
   "id": "715ced8c",
   "metadata": {},
   "source": [
    "The second order ODE above has the general solution\n",
    "\n",
    "$$X = A\\cos(x) + B\\sin(x) = Ae^{ix} + Be^{-ix}$$"
   ]
  },
  {
   "cell_type": "markdown",
   "id": "3b8e44e6",
   "metadata": {},
   "source": [
    "Apply initial conditions $\\theta(0) = 1, \\theta'(0) \\equiv \\frac{d\\theta}{d\\xi}|_{\\xi=0} = 0$"
   ]
  },
  {
   "cell_type": "markdown",
   "id": "496c3b61",
   "metadata": {},
   "source": [
    "$$\\theta(\\xi) = \\frac{A\\cos(\\xi)}{\\xi} + \\frac{B\\sin(\\xi)}{\\xi}$$\n",
    "$$\\theta'(\\xi) = \\frac{-A\\sin(\\xi)\\xi - A\\cos(\\xi)}{\\xi^2} + \\frac{B\\cos(\\xi)\\xi - B\\sin(\\xi)}{\\xi^2}$$\n",
    "$$ = -\\frac{A\\xi\\sin(\\xi)}{\\xi^2} - \\frac{A\\cos(\\xi)}{\\xi^2} + \\frac{B\\xi\\cos(\\xi)}{\\xi^2} - \\frac{B\\sin(\\xi)}{\\xi^2}$$\n",
    "\n",
    "Initial conditions must be applied by limits, thus the initial conditions are\n",
    "\n",
    "$$\\lim_{\\xi\\to0}\\theta = 1$$\n",
    "$$\\lim_{\\xi\\to0}\\frac{d\\theta}{d\\xi} = 0$$\n",
    "\n",
    "For dynamical boundary condition\n",
    "\n",
    "$$\\lim_{\\xi\\to0}-\\frac{A\\xi\\sin(\\xi)}{\\xi^2} - \\frac{A\\cos(\\xi)}{\\xi^2} + \\frac{B\\xi\\cos(\\xi)}{\\xi^2} - \\frac{B\\sin(\\xi)}{\\xi^2} = 0$$\n",
    "\n",
    "$$\\lim_{\\xi\\to0}- \\frac{A\\cos(\\xi)}{\\xi^2} - \\frac{B\\sin(\\xi)}{\\xi^2} = 0$$\n",
    "\n",
    "$$\\Rightarrow A = 0$$\n",
    "\n",
    "For static boundary condition\n",
    "\n",
    "$$\\lim_{\\xi\\to0}\\frac{A\\cos(\\xi)}{\\xi} + \\frac{B\\sin(\\xi)}{\\xi} = 1$$\n",
    "\n",
    "$$\\Rightarrow B = 1$$\n",
    "\n",
    "So the solution is given by\n",
    "\n",
    "$$\\theta(\\xi) = \\frac{\\sin(\\xi)}{\\xi} = \\text{sinc}(\\xi)$$"
   ]
  },
  {
   "cell_type": "markdown",
   "id": "4d3ee767",
   "metadata": {},
   "source": [
    "## Hand working for n=5, solution for LE"
   ]
  },
  {
   "cell_type": "markdown",
   "id": "45919bdc",
   "metadata": {},
   "source": [
    "$$\\frac 1 {\\xi^2} \\frac d{d\\xi}(\\xi^2\\frac{d\\theta}{d\\xi}) + \\theta^5 = 0$$\n",
    "\n",
    "$$ \\frac d{d\\xi}(\\xi^2\\frac{d\\theta}{d\\xi}) = -\\theta^5 \\xi^2$$"
   ]
  },
  {
   "cell_type": "markdown",
   "id": "20a83ad8",
   "metadata": {},
   "source": [
    "higher order\n",
    "substitution\n",
    "direct integration\n",
    "fourier\n",
    "laplace"
   ]
  },
  {
   "cell_type": "markdown",
   "id": "5e7a50f2",
   "metadata": {},
   "source": [
    "Solution should be by the end\n",
    "\n",
    "$$\\theta(\\xi) = \\frac1{\\sqrt{1+\\frac{\\xi^2}{3}}}$$"
   ]
  },
  {
   "cell_type": "markdown",
   "id": "6d6834f7",
   "metadata": {},
   "source": [
    "### Solve the Lane-Emden equation analytically for n = 0, n = 1 and n = 5."
   ]
  },
  {
   "cell_type": "code",
   "execution_count": null,
   "id": "bfcc0ff5",
   "metadata": {},
   "outputs": [
    {
     "data": {
      "text/latex": [
       "$\\displaystyle θ{\\left(ξ \\right)} = 1 - \\frac{ξ^{2}}{6}$"
      ],
      "text/plain": [
       "Eq(θ(ξ), 1 - ξ**2/6)"
      ]
     },
     "execution_count": 20,
     "metadata": {},
     "output_type": "execute_result"
    }
   ],
   "source": [
    "# 1/xi^2 d/dE (xi^2 dt/dxi) + t^n = 0\n",
    "# t = t(xi), p = p_0 t^n, t(0) = 1, dt/dE |_E=0 = 0\n",
    "\n",
    "n = 0\n",
    "\n",
    "theta = sp.Function('θ')\n",
    "xi = sp.symbols(\"ξ\")\n",
    "dthetadxi = theta(xi).diff(xi)\n",
    "\n",
    "sp.dsolve(1/(xi**2) * (xi**2 * dthetadxi).diff(xi) + theta(xi)**n, theta(xi), ics={theta(0):1, theta(xi).diff(xi).subs(xi, 0) : 0})"
   ]
  },
  {
   "cell_type": "code",
   "execution_count": 28,
   "id": "01930b37",
   "metadata": {},
   "outputs": [
    {
     "data": {
      "text/latex": [
       "$\\displaystyle θ{\\left(ξ \\right)} = C_{2} \\left(\\frac{ξ^{4}}{120} - \\frac{ξ^{2}}{6} + 1\\right) + \\frac{C_{1} \\left(- \\frac{ξ^{6}}{720} + \\frac{ξ^{4}}{24} - \\frac{ξ^{2}}{2} + 1\\right)}{ξ} + O\\left(ξ^{6}\\right)$"
      ],
      "text/plain": [
       "Eq(θ(ξ), C2*(ξ**4/120 - ξ**2/6 + 1) + C1*(-ξ**6/720 + ξ**4/24 - ξ**2/2 + 1)/ξ + O(ξ**6))"
      ]
     },
     "execution_count": 28,
     "metadata": {},
     "output_type": "execute_result"
    }
   ],
   "source": [
    "# 1/xi^2 d/dE (xi^2 dt/dxi) + t^n = 0\n",
    "# t = t(xi), p = p_0 t^n, t(0) = 1, dt/dE |_E=0 = 0\n",
    "\n",
    "n = 1\n",
    "\n",
    "theta = sp.Function('θ')\n",
    "xi = sp.symbols(\"ξ\")\n",
    "dthetadxi = theta(xi).diff(xi)\n",
    "\n",
    "sp.dsolve(1/(xi**2) * (xi**2 * dthetadxi).diff(xi) + theta(xi)**n, theta(xi), ics={theta(0):1, theta(xi).diff(xi).subs(xi, 0) : 0}, hint='2nd_power_series_regular')"
   ]
  },
  {
   "cell_type": "markdown",
   "id": "68179842",
   "metadata": {},
   "source": [
    "### Solve the TOV equation for a constant density ρ(r) = ρ0. Do you think this is a physically valid solution?"
   ]
  },
  {
   "cell_type": "markdown",
   "id": "c38a8de3",
   "metadata": {},
   "source": [
    "Tolman-Oppenheimer-Volkoff equation\n",
    "\n",
    "$$\\frac{dP}{dr} = -\\frac{Gm\\rho}{r^2}(1+\\frac{P}{\\rho c^2})(1+\\frac{4\\pi r^2 P}{mc^2})(1-\\frac{2Gm}{rc^2})^{-1}$$"
   ]
  },
  {
   "cell_type": "markdown",
   "id": "cd6d0ebd",
   "metadata": {},
   "source": [
    "Solving the TOV with $\\rho(r) = \\rho_0$"
   ]
  },
  {
   "cell_type": "markdown",
   "id": "a9660b2e",
   "metadata": {},
   "source": []
  }
 ],
 "metadata": {
  "kernelspec": {
   "display_name": ".venv",
   "language": "python",
   "name": "python3"
  },
  "language_info": {
   "codemirror_mode": {
    "name": "ipython",
    "version": 3
   },
   "file_extension": ".py",
   "mimetype": "text/x-python",
   "name": "python",
   "nbconvert_exporter": "python",
   "pygments_lexer": "ipython3",
   "version": "3.13.7"
  }
 },
 "nbformat": 4,
 "nbformat_minor": 5
}
